TM/LM/StepTM.v
@@ -741,7 +741,7 @@ The machine operates on lists of closures and on a heap, so we need a closure-li
   Qed.
 
 
-  (* I forgot that [WHILE] takes a machine over [option unit] instead of [bool]. But that's no problem since we have [ChangePartition]. *)
+  (* I forgot that [While] takes a machine over [option unit] instead of [bool]. But that's no problem since we have [ChangePartition]. *)
   Coercion bool2optunit := fun b : bool => if b then None else Some tt.
 
   Definition Step : pTM sigStep^+ (option unit) 11 :=
@@ -749,7 +749,7 @@ The machine operates on lists of closures and on a heap, so we need a closure-li
       (If (MatchList sigHClos_fin ⇑ _ @ [|Fin0; Fin3|])
           (MatchPair sigHAd_fin sigPro_fin ⇑ retr_clos_step @ [|Fin3; Fin4|];;
            If (MatchList sigTok_fin ⇑ retr_pro_step @ [|Fin3; Fin5|])
-              (MATCH (MatchTok ⇑ retr_tok_step @ [|Fin5|])
+              (Match (MatchTok ⇑ retr_tok_step @ [|Fin5|])
                      (fun t : option ATok =>
                         match t with
                         | Some lamAT =>
